Remove non-network types in TreeDEM

fstar/api/MLS.fst
@@ -15,8 +15,7 @@ open MLS.TreeSync.Invariants.AuthService
 open MLS.TreeDEM.KeyPackageRef
 open MLS.TreeKEM.Operations
 open MLS.TreeKEM.API.Types
-open MLS.TreeDEM.Message.Types
-open MLS.TreeDEM.Message.Content
+open MLS.TreeDEM.NetworkTypes
 open MLS.TreeDEM.Message.Framing
 open MLS.TreeDEM.Welcome
 open MLS.Utils
@@ -111,10 +110,10 @@ let reset_ratchet_states st =
   )
 #pop-options
 
-val process_proposal: nat -> state -> proposal bytes -> result state
+val process_proposal: nat -> state -> proposal_nt bytes -> result state
 let process_proposal sender_id st p =
   match p with
-  | Add key_package ->
+  | P_add {key_package} ->
     //TODO key package signature check
     let? add_pend = MLS.TreeSync.API.prepare_add st.treesync_state key_package.tbs.leaf_node in
     // TODO AS check
@@ -122,52 +121,51 @@ let process_proposal sender_id st p =
     assume (length #bytes key_package.tbs.leaf_node.data.content = hpke_public_key_length #bytes);
     let (treekem_state, _) = MLS.TreeKEM.API.add st.treekem_state ({public_key = key_package.tbs.leaf_node.data.content;}) in
     return ({ st with treesync_state; treekem_state })
-  | Update leaf_package ->
+  | P_update {leaf_node} ->
     if not (sender_id < pow2 st.treesync_state.levels) then
       error "process_proposal: leaf_ind is greater than treesize"
     else (
-      let? pend_update = MLS.TreeSync.API.prepare_update st.treesync_state leaf_package sender_id in
+      let? pend_update = MLS.TreeSync.API.prepare_update st.treesync_state leaf_node sender_id in
       // TODO AS check
       let treesync_state = MLS.TreeSync.API.finalize_update pend_update () in
-      assume (length #bytes leaf_package.data.content = hpke_public_key_length #bytes);
+      assume (length #bytes leaf_node.data.content = hpke_public_key_length #bytes);
       assume(st.treesync_state.levels == st.treekem_state.levels);
-      let treekem_state = MLS.TreeKEM.API.update st.treekem_state ({public_key = leaf_package.data.content}) sender_id in
+      let treekem_state = MLS.TreeKEM.API.update st.treekem_state ({public_key = leaf_node.data.content}) sender_id in
       return ({ st with treesync_state; treekem_state })
     )
-  | Remove leaf_index ->
-    if not (leaf_index < pow2 st.treesync_state.levels) then
+  | P_remove {removed} ->
+    if not (removed < pow2 st.treesync_state.levels) then
       error "process_proposal: leaf_index too big"
     else (
       assume(st.treesync_state.levels == st.treekem_state.levels);
-      let? remove_pend = MLS.TreeSync.API.prepare_remove st.treesync_state leaf_index in
+      let? remove_pend = MLS.TreeSync.API.prepare_remove st.treesync_state removed in
       let treesync_state = MLS.TreeSync.API.finalize_remove remove_pend in
-      let treekem_state = MLS.TreeKEM.API.remove st.treekem_state leaf_index in
+      let treekem_state = MLS.TreeKEM.API.remove st.treekem_state removed in
       return ({ st with treesync_state; treekem_state })
     )
   | _ -> error "process_proposal: not implemented"
 
-val process_proposals: state -> nat -> list (proposal bytes) -> result state
+val process_proposals: state -> nat -> list (proposal_nt bytes) -> result state
 let process_proposals st sender_id proposals =
   let sorted_proposals = List.Tot.concatMap (fun x -> x) [
-    List.Tot.filter (Update?) proposals;
-    List.Tot.filter (Remove?) proposals;
-    List.Tot.filter (Add?) proposals;
-    List.Tot.filter (fun x -> match x with | Add _ | Update _ | Remove _ -> false | _ -> true) proposals;
+    List.Tot.filter (P_update?) proposals;
+    List.Tot.filter (P_remove?) proposals;
+    List.Tot.filter (P_add?) proposals;
+    List.Tot.filter (fun x -> match x with | P_add _ | P_update _ | P_remove _ -> false | _ -> true) proposals;
   ] in
   fold_leftM (process_proposal sender_id) st sorted_proposals
 
 #push-options "--ifuel 1"
-val proposal_or_ref_to_proposal: state -> proposal_or_ref bytes -> result (proposal bytes)
+val proposal_or_ref_to_proposal: state -> proposal_or_ref_nt bytes -> result (proposal_nt bytes)
 let proposal_or_ref_to_proposal st prop_or_ref =
   match prop_or_ref with
-  | Proposal prop -> return prop
-  | Reference ref -> error "proposal_or_ref_to_proposal: don't handle references for now (TODO)"
+  | POR_proposal prop -> return prop
+  | POR_reference ref -> error "proposal_or_ref_to_proposal: don't handle references for now (TODO)"
 #pop-options
 
-val process_commit: state -> msg:message_content bytes{msg.content_type = CT_commit} -> message_auth bytes -> result (state & bytes)
-let process_commit state message message_auth =
-  let message: MLS.TreeDEM.Message.Types.message_content bytes = message in
-  let message_content: commit bytes = message.content in
+val process_commit: state -> wire_format_nt -> msg:framed_content_nt bytes{msg.content.content_type = CT_commit} -> framed_content_auth_data_nt bytes CT_commit -> result (state & bytes)
+let process_commit state wire_format message message_auth =
+  let message_content: commit_nt bytes = message.content.content in
   let? sender_id = (
     if not (S_member? message.sender) then
       error "process_commit: sender is not a member"
@@ -176,11 +174,11 @@ let process_commit state message message_auth =
     )
   ) in
   // 0. Process proposals
-  let? proposals = mapM (proposal_or_ref_to_proposal state) message_content.c_proposals in
+  let? proposals = mapM (proposal_or_ref_to_proposal state) message_content.proposals in
   let? state = process_proposals state sender_id proposals in
   // 1. Process update path
   let? state = (
-    match message_content.c_path with
+    match message_content.path with
     | None -> return state
     | Some path ->
       let? group_context = state_to_group_context state in
@@ -203,9 +201,9 @@ let process_commit state message message_auth =
   // 2. Increase epoch -- TODO when should this happen?!!
   let state = { state with epoch = state.epoch + 1 } in
   // 3. Update transcript
-  let? confirmation_tag = (match message_auth.confirmation_tag with | Some x -> return x | None -> error "process_commit: no confirmation tag") in
+  let confirmation_tag = message_auth.confirmation_tag in
   let? confirmed_transcript_hash = MLS.TreeDEM.Message.Transcript.compute_confirmed_transcript_hash
-    message message_auth.signature state.interim_transcript_hash in
+    wire_format message message_auth.signature state.interim_transcript_hash in
   let? interim_transcript_hash = MLS.TreeDEM.Message.Transcript.compute_interim_transcript_hash
     (confirmation_tag <: bytes) confirmed_transcript_hash in
   let state = { state with confirmed_transcript_hash; interim_transcript_hash } in
@@ -214,8 +212,8 @@ let process_commit state message message_auth =
   // 5. Ratchet.
   let? init_secret = MLS.TreeDEM.Keys.secret_epoch_to_init state.epoch_secret in
   let? leaf_secret = (
-    if state.leaf_index = sender_id && (Some? message_content.c_path) then (
-      match List.Tot.assoc ((ps_prefix_to_ps_whole (ps_leaf_node_nt _)).serialize (Some?.v message_content.c_path).leaf_node) state.pending_updatepath with
+    if state.leaf_index = sender_id && (Some? message_content.path) then (
+      match List.Tot.assoc ((ps_prefix_to_ps_whole (ps_leaf_node_nt _)).serialize (Some?.v message_content.path).leaf_node) state.pending_updatepath with
       | Some leaf_secret -> return leaf_secret
       | None -> internal_failure "Can't retrieve my own leaf secret"
     ) else (
@@ -223,7 +221,7 @@ let process_commit state message message_auth =
     )
   ) in
   let? opt_commit_secret = (
-    match message_content.c_path with
+    match message_content.path with
     | None -> return None
     | Some _ ->
       if not (state.leaf_index < pow2 state.treesync_state.levels) then
@@ -377,7 +375,7 @@ let create e cred private_sign_key group_id =
   })
 #pop-options
 
-val send_helper: state -> msg:message_content bytes{msg.wire_format == WF_mls_private_message} → e:entropy { Seq.length e == 4 } → result (state & message_auth bytes & group_message)
+val send_helper: state -> msg:framed_content_nt bytes → e:entropy { Seq.length e == 4 } → result (state & framed_content_auth_data_nt bytes msg.content.content_type & group_message)
 let send_helper st msg e =
   //FIXME
   assume (sign_nonce_length #bytes == 0);
@@ -388,19 +386,18 @@ let send_helper st msg e =
   let? group_context = state_to_group_context st in
   let? confirmation_secret = MLS.TreeDEM.Keys.secret_epoch_to_confirmation st.epoch_secret in
   let? sender_data_secret = MLS.TreeDEM.Keys.secret_epoch_to_sender_data st.epoch_secret in
-  let? auth = message_compute_auth msg st.sign_private_key rand_nonce (Some group_context) confirmation_secret st.interim_transcript_hash in
-  let? msg_network = message_content_to_network msg in
-  let? auth_network = message_auth_to_network auth in
+  let wire_format = WF_mls_private_message in
+  let? auth = message_compute_auth wire_format msg st.sign_private_key rand_nonce (Some group_context) confirmation_secret st.interim_transcript_hash in
   let auth_msg: authenticated_content_nt bytes = {
-    wire_format = WF_mls_private_message;
-    content = msg_network;
-    auth = auth_network;
+    wire_format;
+    content = msg;
+    auth = auth;
   } in
-  let ratchet = if msg.content_type = CT_application then st.application_state else st.handshake_state in
+  let ratchet = if msg.content.content_type = CT_application then st.application_state else st.handshake_state in
   let? ct_new_ratchet_state = message_to_message_ciphertext ratchet rand_reuse_guard sender_data_secret auth_msg in
   let (ct, new_ratchet_state) = ct_new_ratchet_state in
   let msg_bytes = (ps_prefix_to_ps_whole ps_mls_message_nt).serialize (M_mls10 (M_private_message ct)) in
-  let new_st = if msg.content_type = CT_application then { st with application_state = new_ratchet_state } else { st with handshake_state = new_ratchet_state } in
+  let new_st = if msg.content.content_type = CT_application then { st with application_state = new_ratchet_state } else { st with handshake_state = new_ratchet_state } in
   let g:group_message = (st.treesync_state.group_id, msg_bytes) in
   return (new_st, auth, g)
 
@@ -419,9 +416,9 @@ let rec unsafe_mk_randomness #l e =
 // Have to factor out this function otherwise F* typecheck goes mad in `generate_welcome_message`
 // (Error 54) bytes_like bytes is not a subtype of the expected type bytes
 // Yeah thanks, but I don't see where it's relevant?
-val generate_key_package_and_path_secret: state -> msg:message_content bytes{msg.content_type == CT_commit} -> key_package_nt bytes tkt -> result (key_package_nt bytes tkt & option bytes)
+val generate_key_package_and_path_secret: state -> msg:framed_content_nt bytes{msg.content.content_type == CT_commit} -> key_package_nt bytes tkt -> result (key_package_nt bytes tkt & option bytes)
 let generate_key_package_and_path_secret future_state msg new_key_package =
-  let x: option (update_path_nt bytes) = msg.content.c_path in
+  let x: option (update_path_nt bytes) = msg.content.content.path in
   let new_leaf_package = new_key_package.tbs.leaf_node in
   match x with
   | Some _ -> (
@@ -443,10 +440,9 @@ let generate_key_package_and_path_secret future_state msg new_key_package =
     return (new_key_package, None)
   )
 
-val generate_welcome_message: state -> msg:message_content bytes{msg.content_type == CT_commit} -> message_auth bytes -> bool -> new_key_packages:list (key_package_nt bytes tkt) -> bytes -> result (welcome bytes)
-let generate_welcome_message st msg msg_auth include_path_secrets new_leaf_packages e =
-  let? (future_state, joiner_secret) = process_commit st msg msg_auth in
-  let? confirmation_tag = from_option "generate_welcome_message: confirmation tag is missing" msg_auth.confirmation_tag in
+val generate_welcome_message: state -> wire_format_nt -> msg:framed_content_nt bytes{msg.content.content_type == CT_commit} -> framed_content_auth_data_nt bytes CT_commit -> bool -> new_key_packages:list (key_package_nt bytes tkt) -> bytes -> result (welcome bytes)
+let generate_welcome_message st wire_format msg msg_auth include_path_secrets new_leaf_packages e =
+  let? (future_state, joiner_secret) = process_commit st wire_format msg msg_auth in
   let? tree_hash = (
     if not (MLS.TreeSync.TreeHash.tree_hash_pre future_state.treesync_state.tree) then
       error "generate_welcome_message: bad tree hash pre"
@@ -472,7 +468,7 @@ let generate_welcome_message st msg msg_auth include_path_secrets new_leaf_packa
       extensions = []; //TODO handle group context extensions
     };
     extensions = ratchet_tree_bytes;
-    confirmation_tag = confirmation_tag;
+    confirmation_tag = msg_auth.confirmation_tag;
     signer = future_state.leaf_index;
     signature = empty; //Signed afterward
   } in
@@ -487,7 +483,7 @@ let generate_welcome_message st msg msg_auth include_path_secrets new_leaf_packa
   return welcome_msg
 
 #push-options "--ifuel 2 --fuel 2 --z3rlimit 30"
-val generate_update_path: state -> bytes -> list (proposal bytes) -> result (update_path_nt bytes & (bytes & bytes) & bytes)
+val generate_update_path: state -> bytes -> list (proposal_nt bytes) -> result (update_path_nt bytes & (bytes & bytes) & bytes)
 let generate_update_path st e proposals =
   // TODO: MLS' spec impose to exclude newly added leaves from the resolution computation.
   // This is because the path secret is already encrypted to these leaves in the Welcome message
@@ -534,34 +530,43 @@ let generate_update_path st e proposals =
   )
 #pop-options
 
-let message_commit = m:message_content bytes{m.wire_format == WF_mls_private_message /\ m.content_type == CT_commit}
+let message_commit = m:framed_content_nt bytes{m.content.content_type == CT_commit}
 
-val generate_commit: state -> entropy -> list (proposal bytes) -> result (message_commit & state & entropy)
+val generate_commit: state -> entropy -> list (proposal_nt bytes) -> result (message_commit & state & entropy)
 let generate_commit state e proposals =
   let? (update_path, pending, e) = generate_update_path state e proposals in
+  let? epoch = (if state.epoch < pow2 64 then return state.epoch else error "epoch too big") in
+  let? leaf_index = (if state.leaf_index < pow2 32 then return state.leaf_index else error "leaf index too big") in
+  let? proposals = (
+    let res = List.Tot.map POR_proposal proposals in
+    if bytes_length ps_proposal_or_ref_nt res < pow2 30 then return res
+    else error "proposals too big"
+  ) in
   let state = { state with pending_updatepath = pending::state.pending_updatepath} in
-  let msg: message_content bytes = {
-    wire_format = WF_mls_private_message;
+  assert(0 < pow2 30);
+  let msg: framed_content_nt bytes = {
     group_id = state.treesync_state.group_id;
-    epoch = state.epoch;
-    sender = S_member (state.leaf_index);
-    authenticated_data = Seq.empty; //TODO?
-    content_type = CT_commit;
-    content = { c_proposals = (List.Tot.map Proposal proposals); c_path = Some update_path };
+    epoch;
+    sender = S_member leaf_index;
+    authenticated_data = empty #bytes; //TODO?
+    content = {
+      content_type = CT_commit;
+      content = { proposals; path = Some update_path };
+    };
   } in
   return ((msg <: message_commit), state, e)
 
 let add state key_package e =
-  let? kp = from_option "error message if it is malformed" ((ps_prefix_to_ps_whole (ps_key_package_nt tkt)).parse key_package) in
-  let proposals = [ (Add kp) ] in
+  let? key_package = from_option "error message if it is malformed" ((ps_prefix_to_ps_whole (ps_key_package_nt tkt)).parse key_package) in
+  let proposals = [ (P_add {key_package}) ] in
   let? (msg, state, e) = generate_commit state e proposals in
   let? fresh, e = chop_entropy e 4 in
   let? (state, msg_auth, g) = send_helper state msg fresh in
   let? fresh, e = chop_entropy e 32 in
   let rand = fresh in
   assume (hpke_private_key_length #bytes == 32);
-  assert_norm (List.Tot.length [kp] == 1);
-  let? welcome_msg = generate_welcome_message state msg msg_auth false [kp] rand in
+  assert_norm (List.Tot.length [key_package] == 1);
+  let? welcome_msg = generate_welcome_message state WF_mls_private_message msg msg_auth false [key_package] rand in
   let? welcome_msg_network = welcome_to_network welcome_msg in
   let w:welcome_message = (empty #bytes, (ps_prefix_to_ps_whole ps_welcome_nt).serialize welcome_msg_network) in
   return (state, (g,w))
@@ -569,8 +574,9 @@ let add state key_package e =
 let remove state p e =
   match find_first #(option (leaf_node_nt bytes tkt)) (fun olp -> match olp with | Some lp -> lp.data.credential = C_basic p | None -> false) (get_leaf_list state.treesync_state.tree) with
   | None -> error "remove: can't find the leaf to remove"
-  | Some i -> (
-    let proposals = [Remove i] in
+  | Some removed -> (
+    let? removed = (if removed < pow2 32 then return removed else error "removed too big") in
+    let proposals = [P_remove {removed}] in
     let? (msg, state, e) = generate_commit state e proposals in
     let? fresh, e = chop_entropy e 4 in
     let? (state, _, g) = send_helper state msg fresh in
@@ -585,14 +591,18 @@ let update state e =
   return (state, g)
 
 let send state e data =
-  let msg: message_content bytes = {
-    wire_format = WF_mls_private_message;
+  let? epoch = (if state.epoch < pow2 64 then return state.epoch else error "epoch too big") in
+  let? leaf_index = (if state.leaf_index < pow2 32 then return state.leaf_index else error "leaf index too big") in
+  let? data = (if length data < pow2 30 then return data else error "data too big") in
+  let msg: framed_content_nt bytes = {
     group_id = state.treesync_state.group_id;
-    epoch = state.epoch;
-    sender = S_member state.leaf_index;
-    authenticated_data = Seq.empty; //TODO?
-    content_type = CT_application;
-    content = data;
+    epoch;
+    sender = S_member leaf_index;
+    authenticated_data = empty #bytes; //TODO?
+    content = {
+      content_type = CT_application;
+      content = data;
+    };
   } in
   let? (new_state, msg_auth, g) = send_helper state msg e in
   return (new_state, g)
@@ -716,37 +726,33 @@ let process_welcome_message w (sign_pk, sign_sk) lookup =
 let process_group_message state msg =
   let? msg = from_option "process_group_message: can't parse group message"
     ((ps_prefix_to_ps_whole ps_mls_message_nt).parse msg) in
-  let? message, message_auth = (
+  let? (|wire_format, message, message_auth|) = (
     match msg with
     | M_mls10 (M_public_message msg) ->
         let auth_msg = message_plaintext_to_message msg in
-        let? content = network_to_message_content auth_msg.wire_format auth_msg.content in
-        let? auth = network_to_message_auth auth_msg.auth in
-        return (content, auth)
+        return (|WF_mls_public_message, auth_msg.content, auth_msg.auth|)
     | M_mls10  (M_private_message msg) ->
         let? encryption_secret = MLS.TreeDEM.Keys.secret_epoch_to_encryption state.epoch_secret in
         let? sender_data_secret = MLS.TreeDEM.Keys.secret_epoch_to_sender_data state.epoch_secret in
         let? auth_msg = message_ciphertext_to_message state.treesync_state.levels (encryption_secret <: bytes) (sender_data_secret <: bytes) msg in
-        let? content = network_to_message_content auth_msg.wire_format auth_msg.content in
-        let? auth = network_to_message_auth auth_msg.auth in
-        return (content, auth)
+        return ((|WF_mls_private_message, auth_msg.content, auth_msg.auth|) <: (wire_format_nt & msg:framed_content_nt bytes & framed_content_auth_data_nt bytes msg.content.content_type))
     | _ ->
         internal_failure "unknown message type"
   ) in
   // Note: can't do a dependent pair pattern matching, have to nest matches +
   // annotations because of the dependency
-  match message.content_type with
+  match message.content.content_type with
   | CT_proposal  ->
-      let message_content: proposal bytes = message.content in
+      let message_content: proposal_nt bytes = message.content.content in
       begin match message_content with
-      | Add _ -> internal_failure "TODO: proposal (add)"
+      | P_add _ -> internal_failure "TODO: proposal (add)"
       | _ -> internal_failure "TODO: proposal (other)"
       end
   | CT_commit ->
-      let message_content: commit bytes = message.content in
+      let message_content: commit_nt bytes = message.content.content in
       begin match message_content with
-      | { c_proposals = [ Proposal (Add key_package) ]; c_path = _ } ->
-          let? (state, _) = process_commit state message message_auth in
+      | { proposals = [ POR_proposal (P_add {key_package}) ]; path = _ } ->
+          let? (state, _) = process_commit state wire_format message message_auth in
           let leaf_package = key_package.tbs.leaf_node in
           let? identity = (
             match leaf_package.data.credential with
@@ -754,13 +760,13 @@ let process_group_message state msg =
             | _ -> error "process_group_message: unknown certificate type"
           ) in
           return (state, MsgAdd identity)
-      | { c_proposals = [ Proposal (Remove ind) ]; c_path = _ } ->
+      | { proposals = [ POR_proposal (P_remove {removed}) ]; path = _ } ->
           let? leaf_package =
-            if ind < pow2 (state.treesync_state.levels) then
-              from_option "leaf node" (leaf_at state.treesync_state.tree ind)
+            if removed < pow2 (state.treesync_state.levels) then
+              from_option "leaf node" (leaf_at state.treesync_state.tree removed)
             else error "process_group_message: leaf index too big"
           in
-          let? (state, _) = process_commit state message message_auth in
+          let? (state, _) = process_commit state wire_format message message_auth in
           let? identity = (
             match leaf_package.data.credential with
             | C_basic identity -> return identity
@@ -770,7 +776,7 @@ let process_group_message state msg =
       | _ -> internal_failure "TODO: commit (general case)"
       end
   | CT_application ->
-      let data: bytes = message.content in
+      let data: bytes = message.content.content in
       return (state, MsgData data)
   | _ ->
       internal_failure "unknown message content type"
