fstar/treedem/MLS.TreeDEM.Message.Transcript.fst
@@ -2,26 +2,23 @@ module MLS.TreeDEM.Message.Transcript
 
 open Comparse
 open MLS.TreeDEM.NetworkTypes
-open MLS.TreeDEM.Message.Types
-open MLS.TreeDEM.Message.Content
 open MLS.Result
 open MLS.Crypto
 
 val compute_confirmed_transcript_hash:
   #bytes:Type0 -> {|crypto_bytes bytes|} ->
-  message_content bytes -> bytes -> bytes ->
+  wire_format_nt -> framed_content_nt bytes -> bytes -> bytes ->
   result (lbytes bytes (hash_length #bytes))
-let compute_confirmed_transcript_hash #bytes #cb msg signature interim_transcript_hash =
+let compute_confirmed_transcript_hash #bytes #cb wire_format msg signature interim_transcript_hash =
   if not (length signature < pow2 30) then
     internal_failure "compute_confirmed_transcript_hash: signature too long"
-  else if not (msg.content_type = CT_commit) then
+  else if not (msg.content.content_type = CT_commit) then
     internal_failure "compute_confirmed_transcript_hash: should only be used on a commit message"
   else (
-    let? msg_network = message_content_to_network msg in
     let serialized_msg = serialize (confirmed_transcript_hash_input_nt bytes) ({
-      wire_format = msg.wire_format;
-      content = msg_network;
-      signature = signature;
+      wire_format;
+      content = msg;
+      signature;
     }) in
     let hash_input = concat #bytes interim_transcript_hash serialized_msg in
     if not (length hash_input < hash_max_input_length #bytes) then error ""
